Update 1. Removing some prints 2. Cleaning useless files 3. Experimenting with a general congruence for instruction substitution optimisations.
First attempt at creating a congruence lemma to prove const_prop binds the definition of sound state (according to the value analysis) to the congruence lemma.
(congruence_definition_kildall/congruence_proof_kildall)

(Kildall/general_congruence & general_congruence_proof)
Second try attempts to fix this by stating the definition of a sound state as (P m s), taking in the preservation proof (P m s -> stepD m s = st’ -> P m s’) and by stating if the execution of any instruction is equal to the execution to its optimised instruction.

src/coq/optimisations/local_cfg.v
@@ -1,7 +1,7 @@
 Require Import Vellvm.CFG.
 Require Import Vellvm.Ollvm_ast.
 Require Import Equalities.
-
+Require Import List.
 
 
 Record local_pc : Set := mk_localpc { lbk : block_id;  lpt : instr_id }.
@@ -51,6 +51,16 @@ Definition successor_local_pc (c:cfg) (p:local_pc) :=
   end.
 
 
+
+Definition predecessor_local_pc (c:cfg) (p:local_pc) : list local_pc := nil.
+
+
+
+Lemma make_predecessors_correct_2:
+  forall n code instr s,
+  fetch code n = Some instr -> In s (successor_local_pc code n) ->
+  exists l, predecessor_local_pc code s = l /\ In n l.
+Proof. Admitted.
 
 Module local_pcDec <: MiniDecidableType.
   Definition t := local_pc.
