src/coq/optimisations/test.v
@@ -1,0 +1,42 @@
+From mathcomp.ssreflect
+Require Import ssreflect ssrbool ssrnat eqtype ssrfun seq.
+From mathcomp
+Require Import path.
+From Heaps
+Require Import idynamic ordtype finmap pcm unionmap.
+Set Implicit Arguments.
+Unset Strict Implicit.
+Unset Printing Implicit Defensive.
+
+Section Combine.
+
+Parameters (V : eqType).
+Parameter K : ordType.
+Parameter f : V -> V -> V.
+
+Fixpoint _combine_helper (ks : seq K) (m1 m2 acc : union_map K V) :=
+  if ks is k :: ks'
+  then
+    match (find k m1, find k m2) with
+    | (Some v1, Some v2) => k \\-> (f v1 v2) \+ acc
+    | (Some v1, None) => k \\-> v1 \+ acc
+    | (None, Some v2) => k \\-> v2 \+ acc
+    | _ => acc
+    end
+  else acc.
+
+Definition combine m1 m2 :=
+  _combine_helper (undup (keys_of m1 ++ keys_of m2)) m1 m2 Unit.
+
+Theorem combine_valid m1 m2 :
+  valid m1 -> valid m2 -> valid (combine m1 m2).
+Proof.
+(* 
+
+Induction on the keys of the maps, also check
+the induction lemmas um_indf and um_indb.
+
+ *)
+
+
+End Combine.
